src/program_proof/lockservice/proof.v
@@ -28,16 +28,6 @@ Definition locknameN (lockname : u64) := nroot .@ "lock" .@ lockname.
 
   Parameter validLocknames : gmap u64 unit.
 
-Definition own_clerk (ck:val) (srv:loc) (γrpc:RPC_GS) : iProp Σ
-  :=
-  ∃ (ck_l:loc) (cid cseqno : u64),
-    "%" ∷ ⌜ck = #ck_l⌝
-    ∗ "%" ∷ ⌜int.nat cseqno > 0⌝
-    ∗ "Hcid" ∷ ck_l ↦[Clerk.S :: "cid"] #cid
-    ∗ "Hseq" ∷ ck_l ↦[Clerk.S :: "seq"] #cseqno
-    ∗ "Hprimary" ∷ ck_l ↦[Clerk.S :: "primary"] #srv
-    ∗ "Hcrpc" ∷ RPCClient_own cid cseqno γrpc
-.
 
 Definition TryLock_Post : u64 -> bool -> iProp Σ := λ args reply, (⌜reply = false⌝ ∨ (Ps args))%I.
 Definition TryLock_Pre : u64 -> iProp Σ := λ args, ⌜is_Some (validLocknames !! args)⌝%I.
@@ -69,48 +59,6 @@ Lemma tryLock_core_spec (srv:loc) (tryLockArgs:u64) :
 Proof.
 Admitted.
 
-Definition TryLockRequestC := @RPCRequest u64.
-Definition TryLockReplyC := @RPCReply bool.
-
-Lemma TryLock_spec (srv req_ptr reply_ptr:loc) (req:TryLockRequestC) (reply:TryLockReplyC) γrpc γPost :
-{{{ TryLock_spec_pre srv req_ptr reply_ptr req γrpc γPost
-    ∗ "Hreply" ∷ own_reply reply_ptr reply
-}}}
-  LockServer__TryLock #srv #req_ptr #reply_ptr
-{{{ RET #false; ∃ reply', own_reply reply_ptr reply'
-    ∗ ((⌜reply'.(Stale) = true⌝ ∗ RPCRequestStale req γrpc)
-  ∨ RPCReplyReceipt req reply'.(Ret) γrpc)
-}}}.
-Proof.
-  replace (LockServer__TryLock) with (LockServer_Function LockServer__tryLock_core "LockServer__TryLock"); eauto.
-  iIntros (Φ) "Hpre Hpost".
-  iApply (LockServer_Function_spec with "[Hpre]"); eauto.
-  { apply tryLock_core_spec. } 
-  iDestruct "Hpre" as "[Hpre Hreply]". iFrame.
-Qed.
-
-Lemma CallTryLock_spec (srv args reply:loc) (lockArgs:TryLockRequestC) (lockReply:TryLockReplyC) γrpc γPost :
-{{{ "#Hls" ∷ is_lockserver srv γrpc
-    ∗ "#HargsInv" ∷ inv rpcRequestInvN (TryLockRequest_inv lockArgs γrpc γPost)
-    ∗ "#Hargs" ∷ read_request args lockArgs
-    ∗ "Hreply" ∷ own_reply reply lockReply
-}}}
-  CallTryLock #srv #args #reply
-{{{ e, RET e;
-    (∃ lockReply', own_reply reply lockReply'
-    ∗ (⌜e = #true⌝ ∨ ⌜e = #false⌝
-        ∗ (⌜lockReply'.(Stale) = true⌝ ∗ RPCRequestStale lockArgs γrpc
-               ∨ RPCReplyReceipt lockArgs lockReply'.(Ret) γrpc
-             )))
-}}}.
-Proof using Type*.
-  replace (CallTryLock) with (CallFunction LockServer__TryLock "CallTryLock"); eauto.
-  iIntros (Φ) "Hpre Hpost".
-  iApply (CallFunction_spec with "[Hpre]"); eauto; try refine TryLock_spec; eauto.
-  { by rewrite /Persistent; eauto. }
-  { Opaque own_reply. simpl. iNamed "Hpre". iFrame "#";iFrame. }
-Qed.
-
 Lemma Clerk__TryLock_spec ck (srv:loc) (ln:u64) γrpc :
   {{{
        ⌜is_Some (validLocknames !! ln)⌝
@@ -120,129 +68,8 @@ Lemma Clerk__TryLock_spec ck (srv:loc) (ln:u64) γrpc :
     Clerk__TryLock ck #ln
   {{{ v, RET v; ∃(b:bool), ⌜v = #b⌝ ∗ own_clerk ck srv γrpc ∗ (⌜b = false⌝ ∨ Ps ln) }}}.
 Proof using Type*.
-  iIntros (Φ) "[% [Hclerk #Hsrv]] Hpost".
-  iNamed "Hclerk".
-  rewrite H0.
-  wp_lam.
-  wp_pures.
-  wp_loadField.
-  wp_apply (overflow_guard_incr_spec).
-  iIntros (Hincr_safe).
-  wp_seq.
-  repeat wp_loadField.
-  wp_apply (wp_allocStruct); first eauto.
-  iIntros (args) "Hargs".
-  iDestruct (struct_fields_split with "Hargs") as "(HCID&HSeq&HLockname&_)".
-  iMod (readonly_alloc_1 with "HCID") as "#HCID".
-  iMod (readonly_alloc_1 with "HSeq") as "#HSeq".
-  iMod (readonly_alloc_1 with "HLockname") as "#HLockname".
-  wp_apply wp_ref_to; first eauto.
-  iIntros (args_ptrs) "Hargs_ptr".
-  wp_let.
-  wp_loadField.
-  wp_binop.
-  wp_storeField.
-  wp_apply wp_ref_to; first eauto.
-  iIntros (errb_ptr) "Herrb_ptr".
-  wp_let.
-  wp_apply (wp_allocStruct); first eauto.
-  iIntros (reply) "Hreply".
-  wp_pures.
-  iDestruct "Hsrv" as (mu_ptr) "Hsrv". iNamed "Hsrv".
-  iMod (alloc_γrc {| Args:=ln; CID:=cid; rpc.Seq:=cseqno|} _ TryLock_Pre TryLock_Post with "[Hlinv] [Hcrpc] []") as "[Hcseq_own HallocPost]"; eauto.
-  { simpl. word. }
-  iDestruct "HallocPost" as (γP) "[#Hreqinv_init HγP]".
-  wp_apply (wp_forBreak
-              (fun b =>
- (let lockArgs := ({| Args := ln; CID:= cid; rpc.Seq := cseqno|}) in
-    "#Hargs" ∷ read_request args lockArgs
-  ∗ "#Hargsinv" ∷ (inv rpcRequestInvN (TryLockRequest_inv lockArgs γrpc γP))
-  ∗ "Hcid" ∷ ck_l ↦[Clerk.S :: "cid"] #cid
-  ∗ "Hseq" ∷ (ck_l ↦[Clerk.S :: "seq"] #(LitInt (word.add lockArgs.(rpc.Seq) 1)))
-  ∗ "Hprimary" ∷ ck_l ↦[Clerk.S :: "primary"] #srv
-  ∗ "Hargs_ptr" ∷ args_ptrs ↦[refT (uint64T * (uint64T * (uint64T * unitT))%ht)] #args
-  ∗ "Herrb_ptr" ∷ (∃ (err:bool), errb_ptr ↦[boolT] #err)
-  ∗ "Hreply" ∷ (∃ lockReply, own_reply reply lockReply ∗ (⌜b = true⌝ ∨ (⌜lockReply.(Ret) = false⌝ ∨ Ps ln)))
-  ∗ "HγP" ∷ (⌜b = false⌝ ∨ own γP (Excl ()))
-  ∗ ("Hcseq_own" ∷ cid fm[[γrpc.(cseq)]]↦(int.nat (word.add lockArgs.(rpc.Seq) 1)))
-  ∗ ("HΦpost" ∷ ∀ v : val, (∃ rb : bool, ⌜v = #rb⌝ ∗ own_clerk #ck_l srv γrpc ∗ (⌜rb = false⌝ ∨ Ps ln)) -∗ Φ v)
-              ))%I with "[] [-]"); eauto.
-  {
-    iIntros (Ψ).
-    iModIntro.
-    iIntros "Hpre HΨpost".
-    wp_lam.
-    iNamed "Hpre".
-    iDestruct "Herrb_ptr" as (err_old) "Herrb_ptr".
-    wp_load.
-    wp_loadField.
-    iDestruct "Hreply" as (lockReply) "Hreply".
-    (* WHY: Why does this destruct not work when inside the proof for CalTryLock's pre? *)
-    wp_apply (CallTryLock_spec with "[Hreply]"); eauto.
-    {
-      iSplitL "".
-      { iExists _. iFrame "#". }
-      iFrame "#".
-      iDestruct "Hreply" as "[Hreply rest]".
-      iFrame.
-    }
-
-    iIntros (err) "HCallTryLockPost".
-    iDestruct "HCallTryLockPost" as (lockReply') "[Hreply [#Hre | [#Hre HCallPost]]]".
-    { (* No reply from CallTryLock *)
-      iDestruct "Hre" as %->.
-      wp_store.
-      wp_load.
-      wp_pures.
-      iApply "HΨpost".
-      iFrame; iFrame "#".
-      iSplitL "Herrb_ptr"; eauto.
-      iExists _; iFrame. by iLeft.
-    }
-    { (* Got a reply from CallTryLock *)
-      iDestruct "Hre" as %->.
-      wp_store.
-      wp_load.
-      iDestruct "HγP" as "[%|HγP]"; first discriminate.
-      iDestruct "HCallPost" as "[ [_ Hbad] | #Hrcptstoro]"; simpl.
-      { iDestruct (fmcounter_map_agree_strict_lb with "Hcseq_own Hbad") as %bad. simpl in bad. replace (int.nat (word.add cseqno 1)) with (int.nat cseqno + 1) in bad by word. lia. }
-      iMod (get_request_post with "Hargsinv Hrcptstoro HγP") as "HP".
-      wp_pures.
-      iNamed "Hreply".
-      iApply "HΨpost".
-      iFrame; iFrame "#".
-      iSplitL "Herrb_ptr"; eauto.
-      iSplitR ""; last by iLeft.
-      iExists _; iFrame.
-    }
-  }
-  {
-    iDestruct (struct_fields_split with "Hreply") as "(?& ? & _)".
-    simpl.
-    iFrame; iFrame "#".
-    iSplitL ""; eauto.
-    iSplitL "Herrb_ptr"; eauto.
-    replace (int.nat cseqno + 1) with (int.nat (word.add cseqno 1)) by word.
-    iFrame.
-    Transparent own_reply.
-    iExists {| Ret:=false; Stale:=false |}.  iFrame. by iLeft.
-  }
-
-  iIntros "LoopPost".
-  wp_seq.
-  iNamed "LoopPost".
-  iDestruct "Hreply" as (lockReply) "[Hreply HP]". iNamed "Hreply".
-  iDestruct "HP" as "[%|HP]"; first discriminate.
-  wp_loadField.
-  iApply "HΦpost".
-  iExists lockReply.(Ret); iFrame; iFrame "#".
-  iSplitL ""; first done.
-  unfold own_clerk.
-  iExists _, _, (word.add cseqno 1)%nat; iFrame.
-  simpl.
-  iSplitL ""; first done.
-  assert (int.nat cseqno + 1 = int.nat (word.add cseqno 1))%nat as <-; first by word.
-  iPureIntro. lia.
+  iIntros (Φ) "Hpre Hpost".
+  iApply (Clerk__from_core _ "TryLock" with "[Hpre]"); try apply tryLock_core_spec; eauto.
 Qed.
 
 Lemma Clerk__Lock_spec ck (srv:loc) (ln:u64) γrpc :
